Dfa reloaded, part 1

Cslib/Computability/Dfa/Basic.lean
@@ -6,32 +6,40 @@ Authors: Fabrizio Montesi
 
 import Cslib.Foundations.Semantics.Lts.Basic
 
+/-! # Deterministic Finite-State Automata
+
+A Deterministic Finite-State Automaton (DFA) is a finite-state machine that accepts or rejects
+a finite string.
+-/
+
 /-- A Deterministic Finite-State Automaton (DFA) consists of a labelled transition function
-`tr` over a finite set of states. It has a starting state `start` and a finite
+`tr` over finite sets of states and labels (called symbols), a starting state `start` and a finite
 set of accepting states `accept`. -/
-structure Dfa (State : Type _) (Label : Type _) where
-  -- The transition function of the automaton
-  tr : State → Label → State
-  -- Start state
+structure Dfa (State : Type _) (Symbol : Type _) where
+  /-- The transition function of the automaton. -/
+  tr : State → Symbol → State
+  /-- Start state. -/
   start : State
-  -- Accept states
+  /-- Accept states. -/
   accept : Finset State
-  -- The automaton is finite-state
+  /-- The automaton is finite-state. -/
   finite_state : Finite State
+  /-- The type of symbols (also called 'alphabet') is finite. -/
+  finite_symbol : Finite Symbol
 
 namespace Dfa
 
 /-- `Dfa` is a special case of `Lts`. -/
 @[grind]
-def toLts (dfa : Dfa State Label) : Lts State Label :=
+def toLts (dfa : Dfa State Symbol) : Lts State Symbol :=
   Lts.mk (fun s1 μ s2 => dfa.tr s1 μ = s2)
 
-instance : Coe (Dfa State Label) (Lts State Label) where
+instance : Coe (Dfa State Symbol) (Lts State Symbol) where
   coe := toLts
 
 /-- The LTS induced by a DFA is deterministic. -/
 @[grind]
-theorem toLts_deterministic (dfa : Dfa State Label) : dfa.toLts.Deterministic := by
+theorem toLts_deterministic (dfa : Dfa State Symbol) : dfa.toLts.Deterministic := by
   intro s1 μ s2 s3 htr2 htr3
   by_cases heq : s2 = s3
   case pos => exact heq
@@ -42,29 +50,23 @@ theorem toLts_deterministic (dfa : Dfa State Label) : dfa.toLts.Deterministic :=
 
 /-- The LTS induced by a DFA is finite-state. -/
 @[grind]
-theorem toLts_finiteState (dfa : Dfa State Label) : dfa.toLts.FiniteState :=
+theorem toLts_finiteState (dfa : Dfa State Symbol) : dfa.toLts.FiniteState :=
   dfa.finite_state
 
 /-- A DFA accepts a trace if there is a multi-step accepting derivative with that trace from
 the start state. -/
 @[grind]
-def Accepts (dfa : Dfa State Label) (μs : List Label) :=
+def Accepts (dfa : Dfa State Symbol) (μs : List Symbol) :=
   ∃ s ∈ dfa.accept, dfa.toLts.MTr dfa.start μs s
 
 /-- The language of a DFA is the set of traces that it accepts. -/
 @[grind]
-def language (dfa : Dfa State Label) : Set (List Label) :=
-  fun μs => dfa.Accepts μs
+def language (dfa : Dfa State Symbol) : Set (List Symbol) :=
+  { μs | dfa.Accepts μs }
 
 /-- A trace is accepted by a DFA iff it is in the language of the DFA. -/
 @[grind]
-theorem accepts_mem_language (dfa : Dfa State Label) (μs : List Label) :
-  dfa.Accepts μs ↔ μs ∈ dfa.language := by
-  constructor <;> intro h
-  case mp =>
-    exact h
-  case mpr =>
-    rcases h with ⟨s, h1, h2⟩
-    exists s
+theorem accepts_mem_language (dfa : Dfa State Symbol) (μs : List Symbol) :
+  dfa.Accepts μs ↔ μs ∈ dfa.language := by rfl
 
 end Dfa
